\section{Non-dimensional formulation of the model}
\begin{equation}
D_i=D_i^0,\quad k = \frac{D_0(1+v_sC_s)^\beta}{k_B T c_s} \Rightarrow K=  \frac{D_0(1+v_sC_s)^\beta}{k_B T}.
\end{equation}

Variables rescaling:
\begin{equation*}
\begin{aligned}
k_BT\hat{\mu} + \mu_0 -k_BT= \mu, \qquad \hat{C}_i = vC_i, \qquad \hat{\Phi} = \frac{\Phi e}{k_B T}, \qquad  G_1\hat{p}= p\\
G_1\hat{\mathbb{T}}=\mathbb{T}, \qquad\hat{\mathbf{x}} L =\mathbf{x}, \qquad \hat{t}\tau=t, \qquad e\hat{Q} =v Q, \qquad \hat{K} = \frac{k_BT}{D_0}K\\
\hat{\mathbf{j}}=\frac{vL}{D_0}\mathbf{j}, \qquad \hat{\LL}= \tau \LL
\end{aligned}
\end{equation*}
We also need to rewrite the problem in terms of the current configuration, so that the governing equation become:
\begin{eqnarray}
\partial_t c_s + c_s tr(\LL)=-\nabla \cdot\mathbf{j}_s,\\
\partial_t c_i + c_i tr(\LL)= -\nabla\cdot\mathbf{j}_i,\\
\mathbf{j}_s =-c_sK  \left(\nabla \mu_s +\sum_i \frac{C_i}{C_s} \nabla \mu_i\right)\\
\mathbf{j}_i= - \frac{D_ic_i}{k_B T}\nabla \mu_i + c_i\bar{\mathbf{v}}_s
\end{eqnarray}
So that the a-dimensional set of equation is:
\begin{gather}
\begin{aligned}
\mu_s = p \frac{G_1v_s}{k_BT} - \frac{\gamma}{vk_BT L^2} J \nabla^2 C_s + \left[\ln \frac{C_s}{1+C_s} + \frac{1}{1+C_s}\right.\\
\left.\ \ \ \ \ \ +\frac{\chi}{(1+C_s)^2} + \ln \frac{C_s}{\sum_m C_m} \right], 
\end{aligned}\\[2.5mm]
\mu_i = p \frac{G_1v_i}{k_BT} + \Phi z_i + \ln \frac{C_i}{\sum_m C_m} ,\\
-\frac{\epsilon k_B Tv}{L^2e^2} J \nabla^2 \Phi = Q\, \\
\begin{aligned}
\mathbb{T}= -p \mathbb{I} +\frac{\gamma }{G_1v^2L^2} \left[\frac{1}{2} |\nabla C_s|^2\mathbb{I} - \nabla C_s \otimes \nabla C_s\right]+ J^{-1}\left(\mathbb{B}-\mathbb{I}\right)\\
+ \frac{\epsilon (k_BT)^2}{G_1L^2e^2} \left[\frac{1}{2} \,|\nabla \Phi|^2\mathbb{I} -\nabla \Phi \otimes \nabla \Phi\right],
\end{aligned}\\
\nabla \cdot \mathbb{T}=\mathbf{0}\\
\partial_t c_s + c_s tr(\LL)=- \frac{\tau D_0}{L^2}\nabla \cdot\mathbf{j}_s,\\
\partial_t c_i + c_i tr(\LL)= -\frac{\tau D_0}{L^2}\nabla\cdot\mathbf{j}_i,\\
\mathbf{j}_s =-c_sK  \left(\nabla \mu_s +\sum_i \frac{C_i}{C_s} \nabla \mu_i\right)\\
\mathbf{j}_i= - \frac{D_ic_i}{D_0}\nabla \mu_i + \frac{c_i}{c_s}\mathbf{j}_s
\end{gather}

We consider a 1D problem of constrained swelling, so that the problem simplifies:
\begin{equation}
L_d=\sqrt{\frac{\epsilon k_BTv}{e^2}}<<L \Rightarrow \beta=\frac{L^2_d}{L^2} <<1
\end{equation}
We also assume that:
\begin{equation}
L_{int} = \frac{\gamma}{vk_BT}>L_d
\end{equation}
\begin{gather}
\begin{aligned}
\mu_s = p \mathcal{G} - \frac{L^2_{int}}{L^2} J \partial_{zz} C_s + \left[\ln \frac{C_s}{1+C_s} + \frac{1}{1+C_s}\right.\\
\left.\ \ \ \ \ \ +\frac{\chi}{(1+C_s)^2} + \ln \frac{C_s}{\sum_m C_m} \right], 
\end{aligned}\\[2.5mm]
\mu_i = p \mathcal{G}+ \Phi z_i + \ln \frac{C_i}{\sum_m C_m} ,\\
-\beta^2 J \partial_{zz} \Phi = Q\, \\[2.5mm]
\partial_z T_z=0\\
T_z= -p - \frac{L^2_i}{2\mathcal{G}L^2} (\partial_z C_s)^2+ J^{-1}\left(J^2-1\right)-\frac{\beta^2}{2\mathcal{G}}(\partial_z \Phi)^2,\\
\partial_t c_s + c_s tr(\LL)=- \partial_z j_s,\\
\partial_t c_i + c_i tr(\LL)= -\partial_z j_i,\\
j_s =-c_sK  \left(\partial_z \mu_s +\sum_i \frac{c_i}{c_s} \partial_z \mu_i\right)\\
j_i= - \frac{D_ic_i}{D_0}\partial_z \mu_i + \frac{c_i}{c_s}j_s
\end{gather}

where the time $\tau$ can now be defined as $\tau=L^2/D_0$, where $L$ is the original size of the gel. We thus have that in the external layer, electro neutrality must hold. By expanding the solution in terms of $\beta$ we have at the leading order:
\begin{equation}
Q^0=0 \Longrightarrow \begin{cases}
C_f+\sum_i C^0_i z_i=0,&\qquad gel\\
\sum_i c^0_i z_i = 0, &\qquad bath
\end{cases}
\end{equation}
which implies the concentration of the ion in the solution $c^0_i$ can not be continuous across the layer. Assuming that there are only two ion species so that $z_i=+1,-1$. If we now differentiate the equation (94), we obtain that:
\begin{gather}
 \frac{\partial}{\partial z} \left(j_+-j_-\right)=0,\\
 C_+ - C_-=C_f\\
j_s =-c_sK  \left(\partial_z \mu_s +\sum_i \frac{c_i}{c_s} \partial_z \mu_i\right)\\
j_i= - \frac{D_ic_i}{D_0}\partial_z \mu_i + \frac{c_i}{c_s}j_s\\
 \begin{aligned}
 \mu_s = p \mathcal{G} - \frac{L^2_{int}J}{L^2}  \partial_{zz} C_s + \left[\ln \frac{C_s}{1+C_s} + \frac{1}{1+C_s}\right.\\
 \left.\ \ \ \ \ \ +\frac{\chi}{(1+C_s)^2} + \ln \frac{C_s}{\sum_m C_m} \right], 
 \end{aligned}\\[2.5mm]
 \mu_i = p \mathcal{G}+ \Phi z_i + \ln \frac{C_i}{\sum_m C_m} ,\\
 \partial_z T_z=0\\
 T_z= -p - \frac{L^2_i}{2\mathcal{G}L^2}(\partial_z C_s)^2+ J^{-1}\left(J^2-1\right).
\end{gather}
While in the bath we have:
\begin{gather}
\frac{\partial}{\partial z} \left(j_+-j_-\right)=0,\label{first}\\
c_+=c_-=c_0\\
\mu_s = p \mathcal{G}+ \ln c_s ,\\
\mu_i = p \mathcal{G}+ \Phi z_i + \ln c_i ,\\
\partial_z T_z=0 \Rightarrow \partial_z p = 0\\
j_s =-c_s\partial_z \mu_s +\sum_i c_i \partial_z \mu_i\right)\\
j_i= - \frac{D_ic_i}{D_0}\partial_z \mu_i - \frac{c_i}{c_s}j_s\label{last}
\end{gather}
Substituting~(\ref{last}) into (\ref{first}):
\begin{gather}
j_s = -\partial_z c_s - 2\partial_z c_0=0\Rightarrow \partial_t c_s=0,\\
\partial_z \left( \frac{2D}{D_0}c_0 \partial_z \phi\right) = 0 ,\\
\partial_t c_0 = \frac{D}{D_0}\partial_{zz}c_0
\end{gather}
where the first equation is due to the fact that $c_s+2c_0\equiv1$.
If we now rescale the space with respect to $\beta$, we have:
\begin{gather}
\begin{aligned}
\mu_s = p \mathcal{G} - \frac{L^2_{int}J}{L_d^2}\partial_{zz} C_s + \left[\ln \frac{C_s}{1+C_s} + \frac{1}{1+C_s}\right.\\
\left.\ \ \ \ \ \ +\frac{\chi}{(1+C_s)^2} + \ln \frac{C_s}{\sum_m C_m} \right], \label{sub1}
\end{aligned}\\[2.5mm]
\mu_i = p \mathcal{G}+ \Phi z_i + \ln \frac{C_i}{\sum_m C_m} ,\\
- J\partial_{zz}\Phi = Q\, \\[2.5mm]
T_z= -p - \frac{L^2_i}{2\mathcal{G}L_p^2} (\partial_z C_s)^2+ J^{-1}\left(J^2-1\right)-\frac{1}{2\mathcal{G}}(\partial_z \Phi)^2,\label{sub2}\\
\beta\partial_t c_s + \beta c_s \dot{J}J^{-1}=- \partial_z j_s,\\
\beta\partial_t c_i + \beta c_i \dot{J}J^{-1}= -\partial_z j_i,\\
j_s =-c_sK  \left(\partial_z \mu_s +\sum_i \frac{c_i}{c_s} \partial_z \mu_i\right)\\
j_i= - \frac{D_ic_i}{D_0}\partial_z \mu_i + \frac{c_i}{c_s}j_s
\end{gather}
where we have the new parameter $\xi=L_d/L_{int}<<1$. If we expand $C_s$ in term of $\beta$ and $\xi$, with $\beta<\xi$:
\begin{equation}
C_s = C^{(0,0)}_s+ \xi C_s^{(0,1)}+ \xi^2 C_s^{(0,2)} + \beta C^{(1,0)}_s + \beta\xi C^{(1,1)} + \beta^2 C^{(2,0)}+ h.o.t
\end{equation}

Substituting into Equation~(\ref{sub1})-(\ref{sub2}) and imposing $\mu_s\sim O(1)$ we have:
\begin{gather}
\partial_{zz} C^{(0,0)}=\partial_{zz} C^{(0,1)}=\partial_{zz} C^{(1,0)}=0\\
\begin{aligned}
\mu_s = p \mathcal{G} - \partial_{zz} C^{(0,2)}_s - \frac{L_{int}}{L}\partial_{zz} C^{(1,1)}_s- \frac{L^2_{int}}{L^2}\partial_{zz} C^{(2,0)}_s\\
+\left[\ln \frac{C^{(0,0)}_s}{1+C^{(0,0)}_s}+ \frac{1}{1+C^{(0,0)}_s} +\frac{\chi}{(1+C^{(0,0)}_s)^2} + \ln \frac{C^{(0,0)}_s}{J^{(0,0)}-1} \right], 
\end{aligned}\\[2.5mm]
\partial_z C^{(0,0)}_s=0 \Rightarrow C^{(0,0)}_s= const\\
\begin{aligned}
T^{(0,0)}_z= -p^{(0,0)} -(\partial_z C^{(0,1)}_s)^2-\frac{L_{int}}{L}\partial_{z} C^{(1,0)}_s\partial_{z} C^{(0,1)}_s-\frac{L_{int}^2}{L^2}(\partial_{z} C^{(1,0)}_s)^2\\
+  (J^{(0,0)})^{-1}\left((J^{(0,0)})^2-1\right)-\frac{1}{2\mathcal{G}}(\partial_z \Phi^{(0,0)})^2,
\end{aligned}\\[2mm]
\partial_z T^{(0,0)}_z = 0 \Rightarrow \partial_z p^{(0,0)} = \left(\frac{(J^{(0,0)})^2+1}{(J^{(0,0)})^2}\right)\partial_z J^{(0,0)} + \frac{Q}{\mathcal{G}J}\partial_z \Phi^{(0,0)}\\
\partial_z j_s=\partial_z j_+=\partial_z j_- = 0
\end{gather}

In the bath, we have that:

\begin{gather}
\mu_s = p \mathcal{G}+\ln c_s ,\\
\mu_i = p \mathcal{G}+ \Phi z_i + \ln c_i ,\\
- \epsilon_r\partial_{zz}\Phi = Q\, \\
\partial_z T_z=0 \Rightarrow \partial_z p = \frac{Q}{\mathcal{G}}\partial_z \Phi\\
T_z= -p -\frac{\epsilon_r}{2\mathcal{G}}(\partial_z \Phi)^2,\\
\beta\partial_t c_s =- \partial_z j_s,\\
\beta\partial_t c_i = -\partial_z j_i,
\end{gather}

So that at first order the fluxes $j_m$ are constant in the layer, as well as the stress $T_z$. In the bath we thus have that:
\begin{gather}
\begin{aligned}
j^{bath}_s = - 2Q \partial_z \Phi=\lim\limits_{z\rightarrow \infty} j^{bath}_s=0\\
\Rightarrow Q=0, \ \partial_z \Phi=const 
\end{aligned}\\
j^{bath}_\pm = - \frac{D}{D_0} \partial_z c^{bath}_\pm \pm c^{bath}_\pm\frac{D}{D_0}\partial_z \Phi= j^{gel}_\pm \\
-p^{bath}-\frac{\epsilon_r}{2\mathcal{G}}(\partial_z \Phi)^2=T^{gel}_z\label{sub3}
\end{gather}
while in the gel:
\begin{gather}
0 =C^{(0,0)}_s\partial_z \mu^{(0,0)}_s +\sum_i C^{(0,0)}_i \partial_z \mu_i\\
\begin{aligned}
\partial_z \mu_s = \mathcal{G}\left(\frac{(J^{(0,0)})^2+1}{(J^{(0,0)})^2}\right)\partial_z J^{(0,0)} + \frac{Q}{J^{(0,0)}}\partial_z \Phi^{(0,0)}-\frac{\partial_z J^{(0,0)}}{J^{(0,0)}-1}\\
-\partial_z\left(\partial_{zz} C^{(0,2)}_s + \frac{L_{int}}{L}\partial_{zz} C^{(1,1)}_s+ \frac{L^2_{int}}{L^2}\partial_{zz} C^{(2,0)}_s\right)
\end{aligned}\\
\begin{aligned}
\partial_z \mu_\pm = \mathcal{G}\left(\frac{(J^{(0,0)})^2+1}{(J^{(0,0)})^2}\right)\partial_z J^{(0,0)} + \frac{Q\pm J^{(0,0)}}{J^{(0,0)}}\partial_z \Phi^{(0,0)} \\
+ \frac{\partial_z C_\pm^{(0,0)}}{C_\pm^{(0,0)}}-\frac{\partial_z J^{(0,0)}}{J^{(0,0)}-1}
\end{aligned}\\
\begin{aligned}
0 = \mathcal{G}\left(J^{(0,0)}-1\right)\left(\frac{(J^{(0,0)})^2+1}{(J^{(0,0)})^2}\right)\partial_z J^{(0,0)} +\frac{(2Q-C_f)J^{(0,0)}-Q}{J^{(0,0)}}\partial_z \Phi^{(0,0)} \\
-C_s^{(0,0)}\partial_z\left(\partial_{zz} C^{(0,2)}_s + \frac{L_{int}}{L}\partial_{zz} C^{(1,1)}_s+ \frac{L^2_{int}}{L^2}\partial_{zz} C^{(2,0)}_s\right)
\end{aligned}\\ 
\begin{aligned}
j^{gel}_i= - \frac{Dc^{gel}_i}{D_0}\partial_z \mu^{gel}_i = \frac{D}{D_0}\partial_z c^{bath}_i 
\end{aligned}
\end{gather}
Since we have that in the bulk of the gel $j_+-j_-=0$, we have the additional condition that in the bath $\partial \Phi^{gel}=const=0$.
If we assume the bath to be of infinite size so that the concentration derivative goes to zero:
\begin{equation}
\partial_z c_\pm = const = \lim\limits_{z \rightarrow \infty} c^{bath}_\pm=0, \qquad \mu^{bath}_\pm = \ln c_0.
\end{equation}
This implies that the chemical potential is constant in the bath and thus also in the Debye layer. 
As the stress is zero in the outer region of the bath we have that $T_z$ must be zero everywhere in the layer:
\begin{gather}
p^{bath}= -\frac{\epsilon_r}{2\mathcal{G}} (\partial_z \Phi)^2 = 0 \\
\begin{aligned}
p^{gel}=-(\partial_z C^{(0,1)}_s)^2-\frac{L_{int}}{L}\partial_{z} C^{(1,0)}_s\partial_{z} C^{(0,1)}_s-\frac{L_{int}^2}{L^2}(\partial_{z} C^{(1,0)}_s)^2 \\+ J^{-1}(J^2-1)-\frac{1}{2\mathcal{G}} (\partial_z \Phi)^2
\end{aligned}
\end{gather}
So that the chemical potential are constant inside and outside the gel, at first order. Consequently we have that:
\begin{gather}
\mu^{bath}_\pm = p \mathcal{G}+ \Phi z_i + \ln \frac{C_\pm}{J-1} ,\\
- \partial_Z (J^{-1}\partial_Z\Phi) = Q\, 
\end{gather}
If we also assume that $L_{int}^2/L^2_d>>1$ we must have that at first order:
\begin{equation}
\partial_Z(J^{-1}\partial_ZC^0_s)=0 \Rightarrow \partial_Z C^0_s = J const = \alpha J 
\end{equation}
while the continuity of the stress tensor is given by:
\begin{equation}
-p^{bath}-\frac{\epsilon_r}{2v}\frac{(\partial_Z \Phi)^2}{J^2}=-p - \frac{L^2_i}{2\mathcal{G}L_p^2} \alpha^2 + J^{-1}\left(J^2-1\right)-\frac{1}{2v}\frac{(\partial_Z \Phi)^2}{J^2}
\end{equation}
Also at the first order, have continuity of the electrical potential so that:
\begin{equation}
C^0_i = c^{bath}_0(J-1) \exp\left[\Delta p\mathcal{G}-z_i\Delta \Phi\right]
\end{equation}
where $\Delta=(\cdot)_{bath}-(\cdot)_{gel}$.
In the bath instead the governing equations are:
\begin{gather}
\mu^{b}_s = p^b \mathcal{G} - \frac{L^2_{int,b}}{L^2}  \partial_Z (J^{-1} \partial_Z C_s) + \ln \frac{C_s}{\sum_m C_m}, \\
\mu^{b}_i = p^b \mathcal{G}+ \Phi z_i + \ln \frac{C_i}{\sum_m C_m} ,\\
-\beta^2 \tilde{\epsilon} \partial_Z (J_b^{-1}\partial_Z\Phi) = Q_b\, \\[2.5mm]
T_z= -p - \frac{L^2_{int,b}}{2\mathcal{G}L^2} \frac{(\partial_Z C)^2}{J_{b}^2}-\frac{\beta^2}{2v}\tilde{\epsilon} \frac{(\partial_Z \Phi)^2}{J_b^2},\\
\partial_t C_s=\partial_Z \cdot\left[\frac{K}{J^2} \left(C_s\partial_Z \mu_s +\sum_i  C_i \partial_Z \mu_i\right)\right],\\
\partial_t C_i= \partial_Z \cdot\left[ J_{bath}^{-2}